src/Proofs/Sane.v
@@ -1,0 +1,81 @@
+Require Import Coq.Lists.List.
+Require Import coqutil.Map.Interface coqutil.Map.Properties.
+Require Import riscv.Spec.Machine.
+Require Import riscv.Utility.Monads.
+Require Import riscv.Spec.Decode.
+Require Import riscv.Utility.Utility.
+Require Import riscv.Spec.Primitives.
+Require Import riscv.Platform.RiscvMachine.
+Require Import riscv.Platform.Run.
+
+Import ListNotations.
+
+Section Sane.
+
+  Context {W: Words}.
+  Context {Registers: map.map Register word}.
+  Context {mem: map.map word byte}.
+  Context {M: Type -> Type}.
+  Context {MM: Monad M}.
+  Context {RVM: RiscvProgram M word}.
+  Context {PRParams: PrimitivesParams M RiscvMachine}.
+  Context {mcomp_sat_ok: mcomp_sat_spec PRParams}.
+
+  Lemma mcomp_sat_weaken: forall A initialL m (post1 post2: A -> RiscvMachine -> Prop),
+      (forall a mach, post1 a mach -> post2 a mach) ->
+      mcomp_sat m initialL post1 ->
+      mcomp_sat m initialL post2.
+  Proof.
+    intros.
+    rewrite <- (@right_identity M MM A m).
+    eapply spec_Bind.
+    eexists. split.
+    - exact H0.
+    - intros. simpl in *. apply spec_Return. eapply H. assumption.
+  Qed.
+
+  Lemma Return_sane: forall {A: Type} (a: A),
+      mcomp_sane (Return a).
+  Proof.
+    unfold mcomp_sane.
+    intros. eapply spec_Return in H.
+    split.
+    - eauto.
+    - eapply (proj1 (spec_Return _ _ _)).
+      split.
+      + assumption.
+      + exists nil. reflexivity.
+  Qed.
+
+  Lemma Bind_sane: forall {A B: Type} (m: M A) (f: A -> M B),
+      mcomp_sane m ->
+      (forall a, mcomp_sane (f a)) ->
+      mcomp_sane (Bind m f).
+  Proof.
+    intros *.
+    intros S1 S2.
+    unfold mcomp_sane in *.
+    intros.
+    eapply (proj2 (spec_Bind _ _ _ _)) in H.
+    destruct H as (mid & C1 & C2).
+    split.
+    - specialize S1 with (1 := C1). destruct S1 as ((a & middle & S1a) & S1b).
+      specialize C2 with (1 := S1a).
+      specialize S2 with (1 := C2). destruct S2 as ((b & final & S2a) & S2b).
+      eauto.
+    - eapply spec_Bind.
+      exists (fun a middle => mid a middle /\ exists diff1, getLog middle = diff1 ++ getLog st).
+      split.
+      + specialize S1 with (1 := C1). destruct S1 as ((a & middle & S1a) & S1b).
+        exact S1b.
+      + intros. destruct H as (HM & diff1 & E1).
+        specialize C2 with (1 := HM).
+        specialize S2 with (1 := C2). destruct S2 as ((b & final & S2a) & S2b).
+        eapply mcomp_sat_weaken; [|exact S2b].
+        simpl. intros. destruct H as (? & diff2 & E2). split; [assumption|].
+        rewrite E1 in E2.
+        rewrite List.app_assoc in E2.
+        eexists. exact E2.
+  Qed.
+
+End Sane.
